Change approach to event fixpoints: instead of each event type constructor accessing the "ambient events" in order to allow for `EFork`, `EFork` is just introduced through an event transformer applied on the top.

src/handler.v
@@ -2,35 +2,33 @@ From iris.proofmode Require Import proofmode.
 From iris.base_logic.lib Require Import iprop.
 From ITree Require Import ITree.
 From ITree Require Import Eq.
-From ITree Require Import TranslateFacts.
-From iris.itree Require Import event.
 
 (** An [iHandler] is the used-specified "recipe" used to define a custom
 weakest [WPi]. It specifies how to interpret an event logically, given weakest
 preconditions for continuations of the itree.
 *)
-Record iHandler Σ (EF : (Type → Type) → Type → Type) := IHandler {
-  ihandle :> ∀ preE A,
+Record iHandler Σ (E : Type → Type) := IHandler {
+  ihandle :> ∀ A,
       (* Event [e] *)
-      EF preE A
+      E A
       (* Continuation conditions [λ a, ▷ WPi k a @ H; ∅ {{ Φ }}] *)
     → (A → iProp Σ)
       (* Conditions for spawning threads [λ a, ▷ WPi t @ H; ⊤ {{ True }}] *)
-    → (itree preE unit → iProp Σ)
+    → (itree E unit → iProp Σ)
       (* Condition [WPi Vis e k @ H; ∅ {{ Φ }}] *)
     → iProp Σ;
-    mono : ∀ preE A e Φ Φ' s s',
+    mono : ∀ A e Φ Φ' s s',
         (∀ a, Φ a -∗ Φ' a) -∗
       □ (∀ t, s t -∗ s' t) -∗
-      ihandle preE A e Φ s -∗ ihandle preE A e Φ' s';
+      ihandle A e Φ s -∗ ihandle A e Φ' s';
 }.
 Arguments IHandler {_ _} _.
 
-Global Instance handler_ne Σ EF n (H : iHandler Σ EF) preE A :
-  Proper ((=) ==> ((=) ==> dist n) ==> ((=) ==> dist n) ==> dist n) (ihandle _ _ H preE A).
+Global Instance handler_ne Σ E n (H : iHandler Σ E) A :
+  Proper ((=) ==> ((=) ==> dist n) ==> ((=) ==> dist n) ==> dist n) (ihandle _ _ H A).
 Proof.
   intros e1 e2 <- Φ1 Φ2 HΦ s1 s2 Hs.
-  assert (Hmon : ∀ Φ s, (H preE A e1 Φ s ⊣⊢ ∃ Φ' s', (∀ a, Φ' a -∗ Φ a) ∗ □ (∀ a, s' a -∗ s a) ∗ H preE A e1 Φ' s')).
+  assert (Hmon : ∀ Φ s, (H A e1 Φ s ⊣⊢ ∃ Φ' s', (∀ a, Φ' a -∗ Φ a) ∗ □ (∀ a, s' a -∗ s a) ∗ H A e1 Φ' s')).
   - iIntros (Φ s). iSplit.
     * iIntros "HH". iExists Φ, s. iSplitR; first eauto. iSplitR; first eauto. done.
     * iIntros "[%Φ' [%s' [HmonΦ [Hmons HH]]]]". iApply (mono with "[HmonΦ] [Hmons]"); eauto.
@@ -39,25 +37,6 @@ Proof.
     * by apply Hs.
 Qed.
 
-(** Restricts a handler along a morphism of event types. *)
-Program Definition restrictH {Σ EF2} EF1 (H1 : iHandler Σ EF2) `{EF1 --< EF2} : iHandler Σ EF1 :=
-  IHandler (λ preE A e Φ s, H1 preE A (subevent A e) Φ s)%I _.
-Next Obligation.
-  iIntros (????????????) "HΦ Hs". by iApply (mono with "[HΦ]").
-Qed.
-
-(** Asserts that the [iHandler] [H1] is stronger than [H2]. *)
-Definition subH {Σ EF} (H1 H2 : iHandler Σ EF) : iProp Σ :=
-  ∀ preE A e Φ s, H1 preE A e Φ s -∗ H2 preE A e Φ s.
-
-Lemma subH_transitive {Σ EF} (H1 H2 H3 : iHandler Σ EF) :
-  subH H1 H2 -∗
-  subH H2 H3 -∗
-  subH H1 H3.
-Proof.
-  iIntros "Hsub1 Hsub2" (preE A e Φ s) "HH1". iApply "Hsub2". by iApply "Hsub1".
-Qed.
-
 (** [inH H1 H2] means that, on events [E1], [H1] is stronger than [H2]. *)
-Class inH {Σ EF1 EF2} `{f : EF1 --< EF2} (H1 : iHandler Σ EF1) (H2 : iHandler Σ EF2) :=
-  is_inH : ⊢ subH H1 (restrictH EF1 H2).
+Class inH {Σ E1 E2} `{f : E1 -< E2} (H1 : iHandler Σ E1) (H2 : iHandler Σ E2) :=
+  is_inH : ∀ A e Φ s, H1 A e Φ (λ t, s (translate (λ A e', subevent A e') t)) -∗ H2 A (subevent A e) Φ s.
