src/state.v
@@ -4,7 +4,6 @@ From iris.base_logic.lib Require Import ghost_var.
 From iris.base_logic.lib Require Export fancy_updates.
 From iris.itree Require Import handler.
 From iris.itree Require Import wpi.
-From iris.itree Require Import event.
 From ITree Require Import ITree.
 
 Class stateHPreG (Σ : gFunctors) (S : Type) := StateHPreG {
@@ -20,21 +19,14 @@ Global Instance subG_stateHΣ Σ S :
   subG (stateHΣ S) Σ → stateHPreG Σ S.
 Proof. solve_inG. Qed.
 
-(** An event type for stateful programs with concurrency. *)
-Inductive stateEF (S : Type) (preE : Type → Type) : Type → Type :=
+(** An event type for stateful programs. *)
+Inductive stateE (S : Type) : Type → Type :=
   (** Get the global state. *)
-  | EGetState : stateEF S preE S
+  | EGetState : stateE S S
   (** Set the global state. *)
-  | ESetState (x : S) : stateEF S preE unit
-  (** Yield control to another (demonically chosen) thread in the thread-pool. *)
-  | EYield : stateEF S preE unit
-  (** Split the thread into two threads corresponding to the answers [true]
-  and [false]. *)
-  | EFork (t : itree preE unit) : stateEF S preE unit.
+  | ESetState (x : S) : stateE S unit.
 Arguments EGetState {_}.
 Arguments ESetState {_} _.
-Arguments EYield {_}.
-Arguments EFork {_} _.
 
 (** State interpretation predicate which is enforced at every [EYield], [EGet]
 and [ESet]. *)
@@ -44,33 +36,28 @@ Class stateInterp (Σ : gFunctors) (S : Type) := state_interp : S → iProp Σ.
 Definition state_ro {S} `{!stateInterp Σ S} (s : S) : iProp Σ :=
   ∀ s', state_interp s' -∗ state_interp s' ∗ ⌜ s = s' ⌝.
 
-Program Definition stateH {Σ} (S : Type) `{!stateHGS Σ S} `{!stateInterp Σ S} `{!invGS_gen HasNoLc Σ} : iHandler Σ (stateEF S) :=
-  IHandler (λ preE A e,
+(** [iHandler] for [stateE]. *)
+Program Definition stateH {Σ} (S : Type) `{!stateHGS Σ S} `{!stateInterp Σ S} `{!invGS_gen HasNoLc Σ} : iHandler Σ (stateE S) :=
+  IHandler (λ A e,
     match e with
-    | EGetState _    => λ Φ s, (∀ s, state_interp s -∗ (state_interp s ∗ Φ s))
-    | ESetState _ s' => λ Φ s, (∀ s, state_interp s ={∅}=∗ (state_interp s' ∗ Φ tt))
-    | EYield _       => λ Φ s, |={∅, ⊤}=> |={⊤, ∅}=> Φ tt
-    | EFork _ t      => λ Φ s, Φ tt ∗ s t
+    | EGetState    => λ Φ s, (∀ s, state_interp s -∗ (state_interp s ∗ Φ s))
+    | ESetState s' => λ Φ s, (∀ s, state_interp s ={∅}=∗ (state_interp s' ∗ Φ tt))
     end
   )%I _.
 Next Obligation.
-  iIntros (??????? e ????) "HΦwand Hswand". destruct e.
+  iIntros (?????? e ????) "HΦwand Hswand". destruct e.
   - iIntros "Hget" (?) "Hstate". iDestruct ("Hget" with "Hstate") as "[$ HΦ]". by iApply "HΦwand".
   - iIntros "Hset" (?) "Hstate". iDestruct ("Hset" with "Hstate") as ">[$ HΦ]". by iApply "HΦwand".
-  - iIntros "HΦfupd". by iApply "HΦwand".
-  - iIntros "[HΦ Hs]". iSplitL "HΦ HΦwand".
-    * by iApply "HΦwand".
-    * by iApply "Hswand".
 Qed.
 
 Section wp_state.
-  Context {S : Type} `{!stateHGS Σ S} `{!EventFixpoint EF E} `{!invGS_gen HasNoLc Σ}.
+  Context {S : Type} `{!stateHGS Σ S} {E : Type → Type} `{!invGS_gen HasNoLc Σ}.
   Context `{!stateInterp Σ S}.
-  Context {H : iHandler Σ EF} `{stateEF S --< EF} `{inH Σ (stateEF S) EF (stateH S) H}.
+  Context {H : iHandler Σ E} `{stateE S -< E} `{inH Σ (stateE S) E (stateH S) H}.
 
   Lemma wpi_get {R} (k : S → itree E R) (M : coPset) (Φ : R → iProp Σ) :
     (∀ s, state_interp s -∗ state_interp s ∗ ▷ WPi (k s) @ H; M {{ Φ }}) -∗
-    WPi (visF (EGetState E) k) @ H; M {{ Φ }}.
+    WPi (vis EGetState k) @ H; M {{ Φ }}.
   Proof.
     iIntros "Hwp". iApply wpi_vis.
     iApply fupd_mask_intro; first apply empty_subseteq. iIntros "Hfupd". iApply is_inH.
@@ -80,7 +67,7 @@ Section wp_state.
 
   Lemma wpi_set {R} (s' : S) (k : unit → itree E R) (M : coPset) (Φ : R → iProp Σ) :
     (∀ s, state_interp s ={M}=∗ state_interp s' ∗ ▷ WPi (k tt) @ H; M {{ Φ }}) -∗
-    WPi (visF (ESetState E s') k) @ H; M {{ Φ }}.
+    WPi (vis (ESetState s') k) @ H; M {{ Φ }}.
   Proof.
     iIntros "Hwp". iApply wpi_vis.
     iApply fupd_mask_intro; first apply empty_subseteq. iIntros "Hfupd". iApply is_inH.
@@ -89,13 +76,51 @@ Section wp_state.
     iApply fupd_mask_intro; first apply empty_subseteq. iIntros "Hfupd".
     iNext. rewrite -wpi_clear_mask. iMod "Hfupd". by iMod "Hwp".
   Qed.
+End wp_state.
 
-  Lemma wpi_fork {R} (t : itree E unit) (k : unit → itree E R) (M : coPset) (Φ : R → iProp Σ) :
-    (▷ WPi (k tt) @ H; M {{ Φ }} ∗ ▷ WPi t @ H; ⊤ {{ _, True }}) -∗
-    WPi (visF (EFork E t) k) @ H; M {{ Φ }}.
+(** An event type transformer for adding concurrency. *)
+CoInductive threadpoolE (E : Type → Type) : Type → Type :=
+  | EEmit (A : Type) (e : E A) : threadpoolE E A
+  (** Yield control to another (demonically chosen) thread in the thread-pool. *)
+  | EYield : threadpoolE E unit
+  (** Split the thread into two threads corresponding to the answers [true]
+  and [false]. *)
+  | EFork (t : itree (threadpoolE E) unit) : threadpoolE E unit.
+Arguments EYield {_}.
+Arguments EFork {_} _.
+
+Global Instance E_threadpoolE (E : Type → Type) : Subevent E (threadpoolE E) :=
+  { resum := λ A e, EEmit _ A e }.
+
+(** [iHandler] transformer for [threadpoolE]. *)
+Program Definition threadpoolH {Σ E} `{!invGS_gen HasNoLc Σ} (H : iHandler Σ E) : iHandler Σ (threadpoolE E) :=
+  IHandler (λ A e,
+    match e with
+    | EEmit _ _ e' => λ Φ s, H _ e' Φ (λ t, s (translate (EEmit _) t))
+    | EYield       => λ Φ s, |={∅, ⊤}=> |={⊤, ∅}=> Φ tt
+    | EFork t      => λ Φ s, Φ tt ∗ s t
+    end
+  )%I _.
+Next Obligation.
+  iIntros (??????????) "HΦwand #Hswand". destruct e.
+  - iIntros "HH". iApply (mono with "[HΦwand] [Hswand]"); last done.
+    * exact.
+    * iModIntro. iIntros (t) "Hs". by iApply "Hswand".
+  - iIntros "HΦfupd". by iApply "HΦwand".
+  - iIntros "[HΦ Hs]". iSplitL "HΦ HΦwand".
+    * by iApply "HΦwand".
+    * by iApply "Hswand".
+Qed.
+
+Section wp_threadpool.
+  Context {S : Type} `{!invGS_gen HasNoLc Σ} {E : Type → Type} {H : iHandler Σ E}.
+
+  Lemma wpi_fork {R} (t : itree (threadpoolE E) unit) (k : unit → itree (threadpoolE E) R) (M : coPset) (Φ : R → iProp Σ) :
+    (▷ WPi (k tt) @ threadpoolH H; M {{ Φ }} ∗ ▷ WPi t @ threadpoolH H; ⊤ {{ _, True }}) -∗
+    WPi (Vis (EFork t) k) @ threadpoolH H; M {{ Φ }}.
   Proof.
     iIntros "[Hwp1 Hwp2]". iApply wpi_vis.
-    iApply is_inH. rewrite /stateH. iFrame.
+    rewrite /threadpoolH. iFrame.
     iApply fupd_mask_intro; first apply empty_subseteq. iIntros "Hfupd".
     iNext. rewrite -wpi_clear_mask. iMod "Hfupd". by iMod "Hwp1".
   Qed.
@@ -104,13 +129,13 @@ Section wp_state.
   This means that you cannot step over an [EYield] if there are open
   invariants. It amounts to the typical requirement of atomicity in the
   invariant opening rule known from "normal Iris". *)
-  Lemma wpi_yield {R} (k : unit → itree E R) (M : coPset) (Φ : R → iProp Σ) :
-    (▷ WPi (k tt) @ H; ⊤ {{ Φ }}) -∗
-    WPi (visF (EYield E) k) @ H; ⊤ {{ Φ }}.
+  Lemma wpi_yield {R} (k : unit → itree (threadpoolE E) R) (M : coPset) (Φ : R → iProp Σ) :
+    (▷ WPi (k tt) @ threadpoolH H; ⊤ {{ Φ }}) -∗
+    WPi (Vis EYield k) @ threadpoolH H; ⊤ {{ Φ }}.
   Proof.
-    iIntros "Hwp". iApply wpi_vis. iApply is_inH.
-    rewrite /stateH. simpl. iApply fupd_mask_intro_subseteq; first done.
+    iIntros "Hwp". iApply wpi_vis.
+    rewrite /threadpoolH. simpl. iApply fupd_mask_intro_subseteq; first done.
     iApply fupd_mask_intro; first apply empty_subseteq. iIntros "Hfupd".
     iNext. rewrite -wpi_clear_mask. iMod "Hfupd". by iMod "Hwp".
   Qed.
-End wp_state.
+End wp_threadpool.
